feat: prove (a copy of) Alive testcases with proper UB semantics (#1260)
This PR adds a parser and proof automation for the new SLLVM dialect,
based on the existing LLVM parser&proof automation, and incorporating
some new stuff I proposed in #1220.

I copied AliveStatements so I wouldn't interfere with the existing
evaluation, and then semi-manually changed it to
* use the SLLVM dialect (i.e., proper UB semantics)
* instantiate rewrites to 64 bits (as I haven't bothered implementing
MetaSLLVM yet), except for one testcase where bitblasting timed-out for
any width > 7.

All test cases that were proven before are now proven with proper UB
semantics. Two rewrites that we sorried before turned out to just be
plain false (even without UB), so I noted down the counter-example and
ignored those test cases

SSA/Projects/SLLVM/Dialect/Base.lean
@@ -27,10 +27,41 @@ existing LLVM dialect, *but* it refines the semantics to include a proper model
 of (side-effecting) UB.
 -/
 
+/-! ### Dialect definition -/
+
 def SLLVM : Dialect where
   Op := LLVM.Op
   Ty := LLVM.Ty
   m := UBOr
+
+namespace SLLVM
+
+instance : DecidableEq SLLVM.Op := by unfold SLLVM; infer_instance
+instance : DecidableEq SLLVM.Ty := by unfold SLLVM; infer_instance
+instance : ToString SLLVM.Op    := by unfold SLLVM; infer_instance
+instance : ToString SLLVM.Ty    := by unfold SLLVM; infer_instance
+instance : Repr SLLVM.Op        := by unfold SLLVM; infer_instance
+instance : Repr SLLVM.Ty        := by unfold SLLVM; infer_instance
+instance : Lean.ToExpr SLLVM.Op := by unfold SLLVM; infer_instance
+instance : Lean.ToExpr SLLVM.Ty := by unfold SLLVM; infer_instance
+
+instance : TyDenote SLLVM.Ty    := by unfold SLLVM; infer_instance
+instance : Monad SLLVM.m        := by unfold SLLVM; infer_instance
+instance : LawfulMonad SLLVM.m  := by unfold SLLVM; infer_instance
+
+open Qq in instance : DialectToExpr SLLVM where
+  toExprDialect := q(SLLVM)
+  toExprM := q(Id.{0})
+
+@[match_pattern]
+abbrev Ty.bitvec : Nat → SLLVM.Ty :=
+  InstCombine.LLVM.Ty.bitvec
+
+@[simp_denote] theorem toType_bitvec : TyDenote.toType (Ty.bitvec w) = LLVM.IntW w := rfl
+
+end SLLVM
+
+/-! ### Signature -/
 
 open InstCombine.LLVM.Op in
 /-- The signature of each operation is the same as in LLVM. -/
@@ -38,7 +69,7 @@ instance : DialectSignature SLLVM where
   signature op :=
     { DialectSignature.signature (d := LLVM) op with
         effectKind := match op with
-          | udiv .. | sdiv .. => .impure
+          | udiv .. | sdiv .. | urem .. | srem .. => .impure
           | _ => .pure
     }
 
@@ -49,7 +80,9 @@ open InstCombine.LLVM.Op in
 instance : DialectDenote SLLVM where
   denote
   | udiv _ flag => fun (x ::ₕ (y ::ₕ .nil)) _ => LeanMLIR.SLLVM.udiv x y flag
-  | sdiv _ flag => fun (x ::ₕ (y ::ₕ .nil)) _ => LeanMLIR.SLLVM.udiv x y flag
+  | sdiv _ flag => fun (x ::ₕ (y ::ₕ .nil)) _ => LeanMLIR.SLLVM.sdiv x y flag
+  | urem _      => fun (x ::ₕ (y ::ₕ .nil)) _ => LeanMLIR.SLLVM.urem x y
+  | srem _      => fun (x ::ₕ (y ::ₕ .nil)) _ => LeanMLIR.SLLVM.srem x y
   | op => fun args .nil =>
     EffectKind.liftEffect (EffectKind.pure_le _) <|
       DialectDenote.denote (d := LLVM) op args .nil
