SSA/Core/Util/Poison.lean
@@ -41,13 +41,24 @@ def casesOn'.{u} {α : Type} {motive : PoisonOr α → Sort u}
   | .poison => poison
   | .value a => value a
 
-@[simp] theorem value_inj {a b : α} : value a = value b ↔ a = b := by
+@[simp] theorem value_inj {a b : α} :
+    @Eq (no_index _) (value a) (value b) ↔ a = b := by
+    -- ^^ `value a = value b ↔ _`
   constructor
   · rintro ⟨⟩; rfl
   · exact fun h => h ▸ rfl
 
-theorem poison_ne_value (a : α) : poison ≠ value a := by rintro ⟨⟩
-theorem value_ne_poison (a : α) : value a ≠ poison := by rintro ⟨⟩
+theorem poison_ne_value (a : α) :
+    @Ne (no_index _) poison (value a) := by -- `poison ≠ value a`
+  rintro ⟨⟩
+theorem value_ne_poison (a : α) :
+    @Ne (no_index _) (value a) poison := by -- `value a ≠ poison`
+  rintro ⟨⟩
+
+@[simp]
+theorem ite_value_value {c : Prop} [Decidable c] {a b : α} :
+    (if c then value a else value b : no_index _) = value (if c then a else b) := by
+  split <;> rfl
 
 /-! ### Formatting & Priting instances -/
 instance [ToString α] : ToString (PoisonOr α) where
@@ -203,6 +214,40 @@ instance [DecidableRel (· ⊑ · : α → α → _)] :
   | .poison, _ => .isTrue <| by simp
   | .value _, .poison => .isFalse <| by simp
   | .value a, .value b => decidable_of_decidable_of_iff (p := a ⊑ b) <| by simp
+
+
+/-! ### if-then-else -/
+section Ite
+variable {c : Prop} [Decidable c] (a? b? : PoisonOr α) (a : α)
+
+@[simp]
+theorem if_then_poison_isRefinedBy_iff  :
+    (if c then poison else a? : no_index _) ⊑ b? ↔ ¬c → a? ⊑ b? := by
+  split <;> simp [*]
+
+@[simp]
+theorem value_isRefinedBy_if_then_poison_iff :
+    value a ⊑ (if c then poison else b? : no_index _) ↔ ¬c ∧ (value a ⊑ b?) := by
+  split <;> simp [*]
+
+
+/-!
+Fallback theorems for generic if-then-else; other theorems should be preferred
+as they give simpler rhs's for their specialized situations.
+-/
+theorem ite_isRefinedBy_iff {x? y? z? : PoisonOr α} :
+    ite c x? y? ⊑ z?
+    ↔ let c := c
+      (c → x? ⊑ z?) ∧ (¬c → y? ⊑ z?) := by
+  split <;> simp [*]
+
+theorem isRefinedBy_ite_iff {x? y? z? : PoisonOr α} :
+    x? ⊑ ite c y? z?
+    ↔ let c := c
+      (c → x? ⊑ y?) ∧ (¬c → x? ⊑ z?) := by
+  split <;> simp [*]
+
+end Ite
 
 end Refinement
 
